backends/lean/Aeneas/Std/Scalar/Rotate.lean
@@ -12,35 +12,29 @@ open ScalarElab
 /-!
 ## Rotate Left
 -/
-def UScalar.rotate_left {ty} (x : UScalar ty) (shift : U32) : UScalar ty :=
-  ⟨ x.toBitVec.rotateLeft shift.toNat ⟩
 
 /- [core::num::{u8}::rotate_left] -/
 uscalar @[step_pure_def]
-def core.num.«%S».rotate_left : «%S» → U32 → «%S» := @UScalar.rotate_left .«%S»
-
-def IScalar.rotate_left {ty} (x : IScalar ty) (shift : U32) : IScalar ty :=
+def core.num.«%S».rotate_left (x : «%S») (shift : U32) : «%S» :=
   ⟨ x.toBitVec.rotateLeft shift.toNat ⟩
 
 /- [core::num::{u8}::rotate_left] -/
 iscalar @[step_pure_def]
-def core.num.«%S».rotate_left : «%S» → U32 → «%S» := @IScalar.rotate_left .«%S»
+def core.num.«%S».rotate_left (x : «%S») (shift : U32) : «%S» :=
+  ⟨ x.toBitVec.rotateLeft shift.toNat ⟩
 
 /-!
 ## Rotate Left
 -/
-def UScalar.rotate_right {ty} (x : UScalar ty) (shift : U32) : UScalar ty :=
-  ⟨ x.toBitVec.rotateLeft shift.toNat ⟩
 
 /- [core::num::{u8}::rotate_right] -/
 uscalar @[step_pure_def]
-def core.num.«%S».rotate_right : «%S» → U32 → «%S» := @UScalar.rotate_right .«%S»
-
-def IScalar.rotate_right {ty} (x : IScalar ty) (shift : U32) : IScalar ty :=
+def core.num.«%S».rotate_right (x : «%S») (shift : U32) : «%S» :=
   ⟨ x.toBitVec.rotateLeft shift.toNat ⟩
 
 /- [core::num::{u8}::rotate_right] -/
 iscalar @[step_pure_def]
-def core.num.«%S».rotate_right : «%S» → U32 → «%S» := @IScalar.rotate_right .«%S»
+def core.num.«%S».rotate_right (x : «%S») (shift : U32) : «%S» :=
+  ⟨ x.toBitVec.rotateLeft shift.toNat ⟩
 
 end Aeneas.Std
