backends/lean/Aeneas/Std/Scalar/SaturatingOps.lean
@@ -12,37 +12,33 @@ open Result Error ScalarElab
 /-!
 Saturating add: unsigned
 -/
-def UScalar.saturating_add {ty : UScalarTy} (x y : UScalar ty) : UScalar ty :=
-  ⟨ BitVec.ofNat _ (Min.min (UScalar.max ty) (x.toNat + y.toNat)) ⟩
 
 /- [core::num::{u8}::saturating_add] -/
-uscalar def core.num.«%S».saturating_add := @UScalar.saturating_add UScalarTy.«%S»
+uscalar def core.num.«%S».saturating_add (x y : «%S») : «%S» :=
+  ⟨ BitVec.ofNat _ (Min.min «%S».max (x.toNat + y.toNat)) ⟩
 
 /-!
 Saturating add: signed
 -/
-def IScalar.saturating_add {ty : IScalarTy} (x y : IScalar ty) : IScalar ty :=
-  ⟨ BitVec.ofInt _ (Max.max (IScalar.min ty) (Min.min (IScalar.max ty) (x.toInt + y.toInt))) ⟩
 
 /- [core::num::{i8}::saturating_add] -/
-iscalar def core.num.«%S».saturating_add := @IScalar.saturating_add IScalarTy.«%S»
+iscalar def core.num.«%S».saturating_add (x y : «%S») : «%S» :=
+  ⟨ BitVec.ofInt _ (Max.max «%S».min (Min.min «%S».max (x.toInt + y.toInt))) ⟩
 
 /-!
 Saturating sub: unsigned
 -/
-def UScalar.saturating_sub {ty : UScalarTy} (x y : UScalar ty) : UScalar ty :=
-  ⟨ BitVec.ofNat _ (Max.max 0 (x.toNat - y.toNat)) ⟩
 
 /- [core::num::{u8}::saturating_sub] -/
-uscalar def core.num.«%S».saturating_sub := @UScalar.saturating_sub UScalarTy.«%S»
+uscalar def core.num.«%S».saturating_sub (x y : «%S») : «%S» :=
+  ⟨ BitVec.ofNat _ (Max.max 0 (x.toNat - y.toNat)) ⟩
 
 /-!
 Saturating sub: signed
 -/
-def IScalar.saturating_sub {ty : IScalarTy} (x y : IScalar ty) : IScalar ty :=
-  ⟨ BitVec.ofInt _ (Max.max (IScalar.min ty) (Min.min (IScalar.max ty) (x.toInt - y.toInt))) ⟩
 
 /- [core::num::{i8}::saturating_sub] -/
-iscalar def core.num.«%S».saturating_sub := @IScalar.saturating_sub IScalarTy.«%S»
+iscalar def core.num.«%S».saturating_sub (x y : «%S») : «%S» :=
+  ⟨ BitVec.ofInt _ (Max.max «%S».min (Min.min «%S».max (x.toInt - y.toInt))) ⟩
 
 end Aeneas.Std
